

Chapter 3. Direct Methods for Linear Systems.

Section 1. Gauss Elimination Method.

$$\begin{pmatrix} 2 & 1 \\ 1 & 2 \end{pmatrix} \begin{pmatrix} x \\ y \end{pmatrix} = \begin{pmatrix} 3 \\ 3 \end{pmatrix} \rightarrow (2) - (1) \times \frac{1}{2}$$

$$\begin{pmatrix} 2 & 1 \\ 0 & \frac{3}{2} \end{pmatrix} \begin{pmatrix} x \\ y \end{pmatrix} = \begin{pmatrix} 3 \\ \frac{3}{2} \end{pmatrix} \rightarrow \frac{3}{2}y = \frac{3}{2} \Rightarrow y = 1$$

$$2x + y = 3$$

$$\Rightarrow 2x = 3 - y = 2 \Rightarrow x = 1$$

$$A = (a_{ij})_{n \times n} = \begin{pmatrix} a_{11} & a_{12} & \cdots & a_{1n} \\ a_{21} & a_{22} & \cdots & a_{2n} \\ \vdots & \vdots & \ddots & \vdots \\ a_{n1} & a_{n2} & \cdots & a_{nn} \end{pmatrix} \in \mathbb{R}^n$$

Linear System: $Ax = b$ (1).

$$x = \begin{pmatrix} x_1 \\ x_2 \\ \vdots \\ x_n \end{pmatrix} \in \mathbb{R}^n \quad b = \begin{pmatrix} b_1 \\ b_2 \\ \vdots \\ b_n \end{pmatrix} \in \mathbb{R}^n$$

Assume A is invertible

Idea: eliminate the entries in the lower part of the matrix.

For $k = 1, 2, \dots, n-1$ do (as follows)

For $i = k+1, k+2, \dots, n$ do \leftarrow let $l_{ik} = a_{ik}/a_{kk}$

For $j = k, k+1, \dots, n$ do $b_i^{(k+1)} \leftarrow b_i^{(k)} - l_{ik}b_k^{(k)}$

$$a_{ij}^{(k+1)} \leftarrow a_{ij}^{(k)} - l_{ik} a_{kj}^{(k)}$$

$$\begin{pmatrix} a_{11} & a_{12} & \dots & a_{1n} \\ & a_{22}^{(2)} & \dots & a_{2n}^{(2)} \\ & & a_{33}^{(3)} & \dots & a_{3n}^{(3)} \\ & & & \ddots & \\ & & & & a_{nn}^{(n)} \end{pmatrix} \begin{pmatrix} x_1 \\ x_2 \\ \vdots \\ x_n \end{pmatrix} = \begin{pmatrix} b_1 \\ b_2^{(2)} \\ b_3^{(3)} \\ \vdots \\ b_n^{(n)} \end{pmatrix} \quad (2)$$

Assumption: The diagonal entries are always non-zero in the elimination process.
 $a_{kk}^{(k)} \neq 0$.

$$\begin{pmatrix} 0 & 1 \\ 1 & 1 \end{pmatrix} \begin{pmatrix} x \\ y \end{pmatrix} = \begin{pmatrix} 1 \\ 2 \end{pmatrix} \quad (X)$$

The upper right triangular system can be solved by the backward substitution method.

For $k = n, n-1, \dots, 1$, do

$$a_{kk}^{(k)} x_k = b_k^{(k)} - \sum_{j=k+1}^n a_{kj}^{(k)} x_j$$

$$x_k = (b_k^{(k)} - \sum_{j=k+1}^n a_{kj}^{(k)} x_j) / a_{kk}^{(k)} \quad (*).$$

algorithm complexity.

$$O(n^3) + O(n^2).$$

Section 2. LU-decomposition Method.

Decompose A into the product of a lower triangular and an upper triangular matrix.

Denote the lower and upper triangular matrix by L and U , respectively.

$$A = LU \quad \text{with} \quad L = \begin{pmatrix} 1 & & & & \\ l_{21} & 1 & & & \\ l_{31} & l_{32} & 1 & & \\ \vdots & \vdots & \vdots & \ddots & \vdots \\ l_{n1} & l_{n2} & \vdots & \ddots & 1 \end{pmatrix}$$

$$U = \begin{pmatrix} u_{11} & u_{12} & \cdots & \cdots & u_{1n} \\ & u_{22} & \cdots & \cdots & u_{2n} \\ & & \ddots & \ddots & \vdots \\ & & & \ddots & u_{nn} \end{pmatrix}$$

l_{ik}

$$Ax = b \Rightarrow LUx = b.$$

$$\text{Let } Ux = y. \quad \Rightarrow \quad Ly = b.$$

Step 1. solve $Ly = b$ by forward substitution.

$$\begin{pmatrix} 1 & & & \\ l_{21} & 1 & & \\ l_{31} & l_{32} & 1 & \\ \vdots & \vdots & \vdots & \ddots \end{pmatrix} \begin{pmatrix} y_1 \\ y_2 \\ \vdots \\ y_n \end{pmatrix} = \begin{pmatrix} b_1 \\ b_2 \\ \vdots \\ b_n \end{pmatrix} \quad \checkmark$$

$$O(n^2)$$

Step 2, solve $Ux = y$ by backward substitution.

$$\begin{pmatrix} u_{11} & u_{12} & \dots & u_{1n} \\ & u_{22} & \dots & u_{2n} \\ & & \ddots & \\ & & & u_{nn} \end{pmatrix} \begin{pmatrix} x_1 \\ x_2 \\ \vdots \\ x_n \end{pmatrix} = \begin{pmatrix} y_1 \\ y_2 \\ \vdots \\ y_n \end{pmatrix}.$$

$O(n^2)$

$$\begin{pmatrix} a_{11} & a_{12} & \dots & a_{1n} \\ a_{21} & a_{22} & \dots & a_{2n} \\ \vdots & \vdots & \ddots & \vdots \\ a_{n1} & a_{n2} & \dots & a_{nn} \end{pmatrix} = \begin{pmatrix} 1 & & & \\ l_{21} & 1 & & \\ l_{31} & l_{32} & 1 & \\ \vdots & \vdots & \vdots & \ddots & 1 \end{pmatrix} \begin{pmatrix} u_{11} & u_{12} & \dots & u_{1n} \\ & u_{22} & \dots & u_{2n} \\ & & \ddots & \\ & & & u_{nn} \end{pmatrix}$$

$$a_{11} = u_{11} \quad a_{12} = u_{12} \quad a_{1j} = u_{1j} \quad j = 1, 2, \dots, n$$

$$l_{i1} u_{11} = a_{i1} \quad i = 2, 3, \dots, n \Rightarrow u_{i1} = a_{i1} / u_{11}$$

For $k = 1, 2, \dots, n$.

$$u_{kj} = ? \quad a_{kj} = \sum_{m=1}^k l_{km} u_{mj} \quad j = k, k+1, \dots, n$$

$$= u_{kj} + \sum_{m=1}^{k-1} l_{km} u_{mj}$$

$$u_{kj} = a_{kj} - \sum_{m=1}^{k-1} l_{km} u_{mj}$$

$$l_{ik} = ? \quad a_{ik} = \sum_{m=1}^k l_{im} u_{mj}, \quad i = k+1, \dots, n$$

$$b_{ik} \cdot u_{kj} = a_{ik} - \sum_{m=1}^{k-1} \lim u_{mj}$$